FpuProperties.v
@@ -1,14 +1,13 @@
 Require Import Kami.AllNotations FpuKami.Definitions FpuKami.Classify FpuKami.ModClassify.
 
-Lemma equal_expWidth_sigWidth:
-  forall s, 2^s + 4 > s + 2.
-Proof.
-  induction s; simpl; auto.
-  rewrite Nat.add_0_r.
-  pose proof (pow2_zero s).
-  Omega.omega.
-Qed.
+Section Compat.
 
+
+  Set Implicit Arguments.
+
+End Compat.
+    
+  
 Section Properties.
   Variable expWidthMinus2 sigWidthMinus2: nat.
   
@@ -20,13 +19,13 @@ Section Properties.
 
   Variable expWidth_prop: expWidthMinus2 >= 2.
 
-  Variable expWidthMinus2_plus4_gt_sigWidth: pow2 expWidthMinus2 + 4 > sigWidth.
+  Variable expWidthMinus2_plus4_gt_sigWidth: 2 ^ expWidthMinus2 + 4 > sigWidth.
 
   Lemma expWidth_ge_sigWidth:
-    pow2 expWidthMinus1 > sigWidth.
+    2 ^ expWidthMinus1 > sigWidth.
   Proof.
     rewrite ?Nat.pow_add_r; simpl.
-    assert (sth: pow2 expWidthMinus2 >= 4). {
+    assert (sth: 2 ^ expWidthMinus2 >= 4). {
       pose proof (@Nat.pow_le_mono_r 2 _ _ ltac:(lia) expWidth_prop).
       assumption.
     }
@@ -77,7 +76,7 @@ Section Properties.
                     isFiniteNonzero isSubnormal isSigNaNRawFloat_frac isSigNaNRawFloat
           ] in H;
       repeat rewrite ?andb_true_l, ?andb_true_r, ?andb_false_r, ?andb_false_l in H.
-
+    
     Lemma isSpecial_infOrNaN: evalExpr (isSpecial fn) = evalExpr (infOrNaN fn).
     Proof.
       pose proof expWidth_ge_sigWidth as expWidth_ge_sigWidth.
@@ -86,34 +85,46 @@ Section Properties.
       | |- _ = getBool ?P => destruct P; [rewrite e; simpl in *|]
       end.
       - simpl.
-        destruct (weq (wones expWidth) (natToWord expWidth 0)); simpl.
+        destruct (weq _ (wones expWidth) (natToWord expWidth 0)); simpl.
         + pose proof (@wzero_wones expWidth ltac:(lia)).
           congruence.
-        + unfold wzero.
+        + (* unfold wzero. *)
           rewrite wplus_unit.
           simpl.
+          (* a dirty solution, but a solution... *)
+          assert (ZToWord 0 0 = natToWord 0 0) by auto; rewrite !H; clear H.
+          assert (ZToWord 1 0 = natToWord 1 0) by auto; rewrite !H; clear H.
+          (* assert (ZToWord 1 1 = natToWord 1 1) by auto; rewrite !H; clear H. *)
+          (* assert (ZToWord expWidthMinus1 1 = natToWord _ 1) by auto; rewrite !H; clear H. *)
           rewrite combine_wones_WO; [|unfold wzero; intro].
           * simpl.
+            
             rewrite split1_combine_wplus.
             match goal with
-            | |- getBool (weq (split2 _ _ (_ ^+ ?P)) _) = true => rewrite <- (natToWord_wordToNat P)
+            | |- getBool (weq _ (truncMsb (_ ^+ ?P)) _) = true => rewrite <- (natToWord_wordToNat _ P)
             end.
-            rewrite wordToNat_combine.
+            
+            
+            rewrite !wordToNat_combine; try lia.
+            rewrite Nat.pow_0_r, Nat.mul_1_l.
             simpl.
             rewrite Nat.mul_1_r.
             rewrite wordToNat_natToWord_idempotent'.
             -- rewrite wones_natToWord.
+               
                rewrite <- natToWord_plus.
                simpl.
-               assert (sth: pow2 expWidth - 1 + S (pow2 expWidthMinus1) = pow2 expWidth + pow2 expWidthMinus1) by (pose proof (one_le_pow2 expWidth); lia).
+               assert (sth: 2 ^ expWidth - 1 + S (2 ^ expWidthMinus1) = 2 ^ expWidth + 2 ^ expWidthMinus1) by (pose proof (one_le_pow2 expWidth); lia).
                rewrite sth.
                match goal with
-               | |- getBool (weq ?P _) = true => 
-                 rewrite <- (natToWord_wordToNat P)
+               | |- getBool (weq _ ?P _) = true => 
+                 rewrite <- (natToWord_wordToNat _ P)
                end.
+               
                rewrite wordToNat_split2.
-               assert (sth2: pow2 expWidth + pow2 expWidthMinus1 = pow2 expWidthMinus1 + pow2 expWidth) by lia.
+               assert (sth2: 2 ^ expWidth + 2 ^ expWidthMinus1 = 2 ^ expWidthMinus1 + 2 ^ expWidth) by lia.
                rewrite sth2.
+               
                rewrite natToWord_pow2_add.
                rewrite wordToNat_natToWord_idempotent'.
                ** rewrite Nat.div_same; auto.
@@ -123,19 +134,20 @@ Section Properties.
             -- assert (sth: expWidthMinus2 + 1 = S expWidthMinus2) by lia.
                rewrite sth.
                apply one_lt_pow2.
-          * apply (f_equal (split2 _ 1)) in H.
+          * apply (f_equal (@truncMsb 1 _)) in H.
+            
             rewrite split2_combine in *.
+            
             rewrite split2_zero in *.
             unfold natToWord in H; simpl in *.
             discriminate.
       - simpl.
-        unfold wzero; simpl.
         cbn [natToWord].
         rewrite ?wplus_unit.
         match goal with
-        | |- context [weq ?P (NatToWord expWidth 0)] => remember P as f; simpl in f
+        | |- context [weq _ ?P (natToWord expWidth 0)] => remember P as f; simpl in f
         end.
-        assert (sth3: #f <> pow2 expWidth - 1). {
+        assert (sth3: wordToNat _ f <> 2 ^ expWidth - 1). {
           intro.
           apply (f_equal (natToWord expWidth)) in H.
           rewrite natToWord_wordToNat in H.
@@ -143,51 +155,59 @@ Section Properties.
           subst.
           tauto.
         }
-        assert (sth: #f < pow2 expWidth - 1). {
+        
+        assert (sth: wordToNat _ f < 2 ^ expWidth - 1). {
           pose proof (wordToNat_bound f).
           lia.
         }
         clear sth3 Heqf.
-        destruct (weq f (natToWord expWidth 0)); simpl.
+        destruct (weq _ f (natToWord expWidth 0)); subst; simpl.
         + unfold normDist.
           rewrite ?evalExpr_countLeadingZeros.
           simpl.
           rewrite andb_false_iff; left.
-          assert (sth2: pow2 expWidthMinus1 > sigWidthMinus1) by lia.
-          assert (sth2_5: pow2 (expWidth + 1) > sigWidthMinus1) by (assert (helper: expWidth + 1 = 2 + expWidthMinus1) by lia; rewrite helper; simpl; lia).
+          assert (sth2: 2 ^ expWidthMinus1 > sigWidthMinus1) by lia.
+          assert (sth2_5: 2 ^ (expWidth + 1) > sigWidthMinus1) by (assert (helper: expWidth + 1 = 2 + expWidthMinus1) by lia; rewrite helper; simpl; lia).
           match goal with
-          | |- context[countLeadingZerosWord _ ?P] =>
-            pose proof (countLeadingZerosWord_le_len sth2_5 P)
+          | |- context[countLeadingZerosWord _ _ ?P] =>
+            pose proof (countLeadingZerosWord_le_len _ sth2_5 P)
           end.
           match goal with
-          | |- getBool (weq ?P _) = false => rewrite <- (natToWord_wordToNat P)
+          | |- getBool (weq _ ?P _) = false => rewrite <- (natToWord_wordToNat _ P)
           end.
           rewrite ?wordToNat_split2; simpl.
           repeat match goal with
-                 | |- context [combine ?P ?Q] => rewrite <- (natToWord_wordToNat (combine P Q)); rewrite wordToNat_combine; simpl
-                 end.
+          | |- context [wconcat ?P ?Q] => rewrite <- (natToWord_wordToNat _ (wconcat P Q)); rewrite wordToNat_combine; simpl
+          end.
           rewrite ?Nat.mul_1_r, ?Nat.mul_0_r, ?Nat.add_0_r.
           rewrite ?wordToNat_natToWord_idempotent'.
           * rewrite Nat.div_small; simpl; auto.
-            pre_word_omega.
+            (* simpl; rewrite Z.mod_small; try split; try lia; simpl.
+            2:{ rewrite <- Z.pow_1_r at 1.
+                apply Z.pow_lt_mono_r; lia. } *)
+            (* pre_word_omega. *)
             match goal with
-            | |- context [weq ?w1 ?w2] => destruct (weq w1 w2); simpl
+            | |- context [weq _ ?w1 ?w2] => destruct (weq _ w1 w2); simpl
             end.
-            ** assert (sth3: pow2 (expWidth+1) = pow2 (expWidthMinus1) + pow2 (expWidthMinus1) + pow2 expWidth) by (rewrite ?Nat.add_1_r; simpl; lia).
+            ** assert (sth3: 2 ^ (expWidth+1) = 2 ^ (expWidthMinus1) + 2 ^ (expWidthMinus1) + 2 ^ expWidth) by (rewrite ?Nat.add_1_r; simpl; lia).
               rewrite wplus_comm.
               rewrite wneg_wnot.
               rewrite wminus_def.
               rewrite <- wneg_wplus_distr.
+              replace (ZToWord (expWidth + 1) 1) with (natToWord (expWidth + 1) 1); auto.
               rewrite <- natToWord_plus.
+              (* assert (sth_tmp : (1 = Z.of_nat 1)%Z) by auto.
+              rewrite sth_tmp; rewrite <- Nat2Z.inj_add; clear sth_tmp.*)
               rewrite <- wminus_def.
               rewrite wminus_minus.
-              apply lt_minus.
+              (* rewrite Nat2Z_ZToWord.*)
+              apply lt_minus'.
               rewrite ?wordToNat_natToWord_idempotent'; lia.
               rewrite wordToNat_natToWord_idempotent'.
               rewrite Nat.pow_add_r; simpl; lia.
               do 2 rewrite Nat.pow_add_r; simpl. lia.
               rewrite wordToNat_natToWord_idempotent'.
-              assert (sth4: pow2 expWidth = pow2 (expWidthMinus1) + pow2 (expWidthMinus1) ).
+              assert (sth4: 2 ^ expWidth = 2 ^ (expWidthMinus1) + 2 ^ (expWidthMinus1) ).
               rewrite ?Nat.add_1_r; simpl; lia.
               rewrite sth4.
               do 2 rewrite <- Nat.add_1_r.
@@ -200,25 +220,32 @@ Section Properties.
               rewrite Plus.plus_assoc_reverse.
               apply Plus.plus_lt_compat_l.
               lia.
-              pre_word_omega.
-              rewrite ?wordToNat_natToWord_idempotent'; lia.
-            ** rewrite wordToNat_natToWord_idempotent' in H by lia.
-            assert (sth3: sigWidthMinus1 < pow2 expWidthMinus1 - 1) by lia.
-            rewrite wordToNat_wplus.
-            rewrite wordToNat_wnot.
-            rewrite wordToNat_natToWord_idempotent'.
-            -- simpl in *.
-               match type of H with
-               | ?P <= _ => remember P as rem
-               end.
-               assert (sth4: pow2 (expWidth + 1) > rem). {
+              simpl.
+              unfold wltu. unfold natToWord.
+              rewrite !wordToZ_ZToWord; try split; try rewrite <- Zpow_of_nat; try lia.
+              apply Z.ltb_lt; apply Nat2Z.inj_lt; lia.
+            ** unfold wleu, natToWord in H. 
+               rewrite wordToZ_ZToWord in H by (rewrite <- Zpow_of_nat; lia).
+               assert (sth3: sigWidthMinus1 < 2 ^ expWidthMinus1 - 1) by lia.
+               rewrite wordToNat_wplus.
+               rewrite wordToNat_wnot.
+               rewrite wordToNat_natToWord_idempotent'.
+                 -- simpl in *.
+                    apply Z.leb_le in H.
+                    apply Z2Nat.inj_le in H; try apply wordVal_pos; try lia.
+                    rewrite Nat2Z.id in H.
+                    unfold wordToNat.
+                    match type of H with
+                    | ?P <= _ => remember P as rem
+                    end.
+               assert (sth4: 2 ^ (expWidth + 1) > rem). {
                  assert (helper: expWidth + 1 = 2 + expWidthMinus1) by lia.
                  rewrite helper.
                  simpl; lia.
                }
                pose proof (one_le_pow2 (expWidth + 1)) as sth5.
-               assert (sth6: rem < pow2 expWidthMinus1) by lia.
-               assert (sth7: pow2 (expWidth + 1) - rem - 1 + S (S (pow2 expWidthMinus1)) = pow2 (expWidth + 1) + (S (pow2 expWidthMinus1) - rem)) by lia.
+               assert (sth6: rem < 2 ^ expWidthMinus1) by lia.
+               assert (sth7: 2 ^ (expWidth + 1) - rem - 1 + S (S (2 ^ expWidthMinus1)) = 2 ^ (expWidth + 1) + (S (2 ^ expWidthMinus1) - rem)) by lia.
                rewrite sth7.
                rewrite Nat.add_mod by lia.
                rewrite Nat.mod_same by lia; simpl.
@@ -229,38 +256,67 @@ Section Properties.
             -- rewrite ?Nat.pow_add_r; simpl.
                pose proof (zero_lt_pow2 expWidthMinus2).
                lia.
-          * clear f fn n sth e H.
-            destruct expWidthMinus1; lia.
-          * assert (sth3: pow2 expWidth = pow2 (S expWidthMinus1)) by (f_equal; lia).
-            rewrite sth3; simpl.
-            rewrite wordToNat_natToWord_idempotent'; lia.
-        + rewrite <- (natToWord_wordToNat (combine f (NatToWord 1 0))).
-          rewrite <- (natToWord_wordToNat (combine (combine (NatToWord expWidthMinus1 1) WO~1) (NatToWord 1 0))).
-          rewrite ?wordToNat_combine.
+                 * rewrite <- Nat.pow_1_r at 1.
+                   apply Nat.pow_lt_mono_r; lia.
+                 * unfold wordToNat. simpl.
+                   apply Nat2Z.inj_lt.
+                   rewrite Z2Nat.id.
+                   rewrite Zpow_of_nat.
+                   apply Z_mod_lt.
+                   rewrite <- Zpow_of_nat. lia.
+                   apply Z.mod_pos_bound.
+                   rewrite <- Zpow_of_nat. lia.
+                 * unfold wordToNat. simpl.
+                   rewrite Z2Nat.id.
+                   rewrite Z.mod_mod.
+                   rewrite Z.mod_small.
+                   rewrite !pow2_add_mul.
+                   simpl.
+                   assert (sth3: 2 < 2 ^ expWidthMinus2).
+                   rewrite <- Nat.pow_1_r at 1.
+                   apply Nat.pow_lt_mono_r; lia.
+                   lia.
+                   split; try lia.
+                   apply Z2Nat.inj_lt; try lia.
+                   apply Z.pow_nonneg; lia.
+                   rewrite <- Zpow_of_nat, Nat2Z.id.
+                   assert (th: Z.to_nat 2 = 2); auto; rewrite th; clear th.
+                   rewrite <- Nat.pow_1_r at 1.
+                   apply Nat.pow_lt_mono_r; lia.
+                   apply Z.pow_nonzero; lia.
+                   apply Z.mod_pos_bound.
+                   apply Z.pow_pos_nonneg; lia.
+                 * auto.
+                 * auto.
+                 * auto.
+        + rewrite <- (natToWord_wordToNat _ (wconcat (natToWord 1 0) f)).
+          rewrite <- (natToWord_wordToNat _ (wconcat (ZToWord 1 0)
+            (wconcat (ZToWord 1 1) (wconcat (ZToWord expWidthMinus1 1) (ZToWord 0 0))))).
+          rewrite ?wordToNat_combine; auto.
           simpl.
           rewrite ?Nat.mul_0_r, ?Nat.add_0_r, ?Nat.mul_1_r.
           rewrite wordToNat_natToWord_idempotent' with (n := 1) by lia.
           rewrite <- natToWord_plus.
           match goal with
-          | |- getBool (weq ?P _) && getBool (weq ?Q _) = false => rewrite <- (natToWord_wordToNat P);
-                                                                     rewrite <- (natToWord_wordToNat Q)
+          | |- getBool (weq _ ?P _) && getBool (weq _ ?Q _) = false => rewrite <- (natToWord_wordToNat _ P);
+                                                                     rewrite <- (natToWord_wordToNat _ Q)
           end.
           rewrite ?wordToNat_split2; simpl.
           rewrite wordToNat_split1; simpl.
-          assert (sth1: pow2 expWidth >= 1) by lia.
-          assert (sth2: #f + S (pow2 expWidthMinus1) < pow2 (expWidth + 1)). {
+          assert (sth1: 2 ^ expWidth >= 1) by lia.
+          assert (sth2: wordToNat _ f + S (2 ^ expWidthMinus1) < 2 ^ (expWidth + 1)). {
             assert (sth3: S expWidth = expWidth + 1) by lia; rewrite <- sth3; simpl.
-            assert (sth4: pow2 (S expWidthMinus1) = pow2 expWidth) by (f_equal; lia).
+            assert (sth4: 2 ^ (S expWidthMinus1) = 2 ^ expWidth) by (f_equal; lia).
             rewrite <- sth4 in *; simpl.
             simpl in *.
             lia.
           }
           rewrite ?wordToNat_natToWord_idempotent' by auto.
           rewrite andb_false_iff.
-          assert (sth3: pow2 expWidthMinus1 >= 1) by lia.
-          assert (sth4: pow2 expWidth = pow2 (S expWidthMinus1)) by (f_equal; lia).
-          destruct (Compare_dec.le_lt_dec (pow2 expWidthMinus1-1) (#f)); [ right | left].
-          * rewrite mod_sub; simpl; rewrite ?Nat.add_0_r; try nia.
+          assert (sth3: 2 ^ expWidthMinus1 >= 1) by lia.
+          assert (sth4: 2 ^ expWidth = 2 ^ (S expWidthMinus1)) by (f_equal; lia).
+          destruct (Compare_dec.le_lt_dec (2 ^ expWidthMinus1-1) (wordToNat _ f)); [ right | left ].
+          * rewrite mod_sub'; simpl; rewrite ?Nat.add_0_r; try nia.
             -- rewrite Nat.div_small; simpl; auto.
                rewrite sth4 in *; simpl in *.
                nia.
@@ -279,14 +335,14 @@ Section Properties.
       apply andb_false_intro1.
       simpl in *.
       match goal with
-      | H: getBool (weq ?P ?Q) = true |- getBool (weq ?P ?R) = false => destruct (weq P Q) as [p|q]; [rewrite p; simpl |]
+      | H: getBool (weq _ ?P ?Q) = true |- getBool (weq _ ?P ?R) = false => destruct (weq _ P Q) as [p|q]; [rewrite p; simpl |]
       end.
-      - destruct (weq (natToWord expWidth 0) (wones expWidth)); auto.
+      - destruct (weq _ (natToWord expWidth 0) (wones expWidth)); auto.
         exfalso.
         apply wzero_wones in e; auto.
         lia.
       - simpl in *; discriminate.
-    Qed.
+    Qed. 
 
     Lemma isZero_not_infOrNaN: evalExpr (isZero fn) = true -> evalExpr (infOrNaN fn) = false.
     Proof.
@@ -315,7 +371,7 @@ Section Properties.
     Qed.
 
     Lemma infOrNaN_sExp_expWidthMinus2':
-      evalExpr (infOrNaN fn) = true -> getBool (weq (evalExpr (sExp_expWidthMinus2 (getRawFloat_from_FN fn))) WO~0) = true.
+      evalExpr (infOrNaN fn) = true -> getBool (weq _ (evalExpr (sExp_expWidthMinus2 (getRawFloat_from_FN fn))) WO~0) = true.
     Proof.
       pose proof expWidth_ge_sigWidth as expWidth_ge_sigWidth.
       simpl.
@@ -324,11 +380,11 @@ Section Properties.
       match type of H with
       | getBool ?P = _ => destruct P
       end; simpl in *; [clear H; rewrite e; clear e| discriminate].
-      destruct (weq (wones expWidth) (NatToWord expWidth 0)); simpl; [pose proof (@wzero_wones expWidth ltac:(lia)); congruence| clear n].
+      destruct (weq _ (wones expWidth) (natToWord expWidth 0)); simpl; [pose proof (@wzero_wones expWidth ltac:(lia)); congruence| clear n].
       rewrite wzero_wplus.
       match goal with
-      | |- getBool (weq (split2 _ _ (split1 _ _ (split1 _ _ ?P))) _) = true =>
-        rewrite <- (natToWord_wordToNat P)
+      | |- getBool (weq _ (@truncMsb _ _ (@truncLsb _ _ (@truncLsb _ _ ?P))) _) = true =>
+        rewrite <- (natToWord_wordToNat _ P)
       end.
       rewrite wordToNat_wplus.
       rewrite ?wordToNat_combine.
@@ -338,34 +394,38 @@ Section Properties.
       rewrite wordToNat_natToWord_idempotent' by lia.
       assert (sth0: expWidth + 1 = S expWidth) by lia.
       assert (sth1: expWidth = S expWidthMinus1) by lia.
-      assert (sth2: pow2 expWidth >= 1) by (rewrite sth1; pose proof (one_lt_pow2 expWidthMinus1); lia).
-      assert (sth3: pow2 expWidth - 1 + (1 + pow2 expWidthMinus1) = pow2 expWidth + pow2 expWidthMinus1) by lia.
+      assert (sth2: 2 ^ expWidth >= 1) by (rewrite sth1; pose proof (one_lt_pow2 expWidthMinus1); lia).
+      assert (sth3: 2 ^ expWidth - 1 + (1 + 2 ^ expWidthMinus1) = 2 ^ expWidth + 2 ^ expWidthMinus1) by lia.
       rewrite sth3.
       rewrite Nat.mod_small by (rewrite sth0, sth1; simpl; lia).
       match goal with
-      | |- getBool (weq (split2 _ _ (split1 _ _ ?P)) _) = _ =>
-        rewrite <- (natToWord_wordToNat P)
+      | |- getBool (weq _ (@truncMsb _ _ (@truncLsb _ _ ?P)) _) = _ =>
+        rewrite <- (natToWord_wordToNat _ P)
       end.
       rewrite wordToNat_split1.
       rewrite wordToNat_natToWord_idempotent' by (rewrite sth0, sth1; simpl; lia).
-      assert (sth4: pow2 expWidth + pow2 expWidthMinus1 = pow2 expWidthMinus1 + 1 * pow2 expWidth) by lia.
+      assert (sth4: 2 ^ expWidth + 2 ^ expWidthMinus1 = 2 ^ expWidthMinus1 + 1 * 2 ^ expWidth) by lia.
       rewrite sth4.
       rewrite Nat.mod_add by lia.
       rewrite Nat.mod_small by (rewrite sth1; simpl; lia).
       match goal with
-      | |- getBool (weq (split2 _ _ ?P) _) = _ =>
-        rewrite <- (natToWord_wordToNat P)
+      | |- getBool (weq _ (@truncMsb _ _ ?P) _) = _ =>
+        rewrite <- (natToWord_wordToNat _ P)
       end.
       rewrite wordToNat_split1.
       rewrite wordToNat_natToWord_idempotent' by (rewrite sth1; simpl; lia).
       rewrite Nat.mod_same by lia.
       match goal with
-      | |- getBool (weq ?P _) = _ =>
-        rewrite <- (natToWord_wordToNat P)
+      | |- getBool (weq _ ?P _) = _ =>
+        rewrite <- (natToWord_wordToNat _ P)
       end.
       rewrite wordToNat_split2.
       rewrite wordToNat_natToWord_idempotent' by lia.
       rewrite Nat.div_0_l by (pose proof (zero_lt_pow2 expWidthMinus2); lia).
+      auto.
+      auto.
+      auto.
+      auto.
       auto.
     Qed.
 
@@ -374,7 +434,7 @@ Section Properties.
     Proof.
       intros H.
       apply infOrNaN_sExp_expWidthMinus2' in H.
-      destruct (weq (evalExpr (sExp_expWidthMinus2 (getRawFloat_from_FN fn))) WO~0); [auto|discriminate].
+      destruct (weq _ (evalExpr (sExp_expWidthMinus2 (getRawFloat_from_FN fn))) WO~0); [auto|discriminate].
     Qed.
 
     Lemma isNaN_or_Inf_infOrNaN:
@@ -390,21 +450,9 @@ Section Properties.
       rewrite ?split1_combine.
       auto.
     Qed.
-
-    Lemma getBool_weq sz (w1 w2: word sz):
-      getBool (weq w1 w2) = true -> w1 = w2.
-    Proof.
-      intros.
-      destruct (weq w1 w2); [auto | discriminate].
-    Qed.
-
-    Lemma if_same A (x: A) (p: bool): (if p then x else x) = x.
-    Proof.
-      destruct p; auto.
-    Qed.
     
     Lemma infOrNaN_isZeroNaNInf2_0_isZeroFractIn:
-      evalExpr (infOrNaN fn) = true -> getBool (weq (evalExpr (isZeroNaNInf2 (getRecFN_from_FN fn))) WO~0) = evalExpr (isZeroFractIn fn).
+      evalExpr (infOrNaN fn) = true -> getBool (weq _ (evalExpr (isZeroNaNInf2 (getRecFN_from_FN fn))) WO~0) = evalExpr (isZeroFractIn fn).
     Proof.
       intros sth1.
       pose proof isSpecial_infOrNaN as sth2.
@@ -413,6 +461,7 @@ Section Properties.
       rewrite sth3.
       rewrite sth2.
       rewrite sth1.
+      clear sth2 sth3.
       rewrite if_same.
       rewrite wor_wzero.
       rewrite andb_true_l.
@@ -422,7 +471,7 @@ Section Properties.
     Qed.
 
     Lemma infOrNaN_isZeroNaNInf2_1_isZeroFractIn:
-      evalExpr (infOrNaN fn) = true -> getBool (weq (evalExpr (isZeroNaNInf2 (getRecFN_from_FN fn))) WO~1) = negb (evalExpr (isZeroFractIn fn)).
+      evalExpr (infOrNaN fn) = true -> getBool (weq _ (evalExpr (isZeroNaNInf2 (getRecFN_from_FN fn))) WO~1) = negb (evalExpr (isZeroFractIn fn)).
     Proof.
       intros sth1.
       pose proof isSpecial_infOrNaN as sth2.
@@ -478,35 +527,7 @@ Section Properties.
       auto.
     Qed.
 
-    Lemma mod_factor' a b c d:
-      b <> 0 -> c <> 0 -> d = b * c -> (a mod d) mod b = a mod b.
-    Proof.
-      pose proof (@mod_factor a b c).
-      intros.
-      subst.
-      eapply H; eauto.
-    Qed.
-
-    Lemma mod_sub a b c:
-      c > 0 ->
-      a >= b * c ->
-      (a - b * c) mod c = a mod c.
-    Proof.
-      intros.
-      assert (sth: a - b * c + b * c = a) by lia.
-      rewrite <- sth at 2.
-      rewrite Nat.mod_add by lia.
-      auto.
-    Qed.
-
-    Lemma split1_fits_natToWord n sz:
-      n < pow2 sz -> 
-      (split1 sz 1 (NatToWord (sz + 1) n) = NatToWord sz n).
-    Proof.
-      intro.
-      rewrite <- combine_natToWord_wzero; auto.
-      rewrite split1_combine;auto. 
-    Qed.
+    (* copy-pasted from bbv, commit b98e19b *)
 
     Lemma isZeroRecFN_isZero:
       evalExpr (isZeroRecFN (getRecFN_from_FN fn)) = evalExpr (isZero fn).
@@ -539,35 +560,35 @@ Section Properties.
           | |- context [if getBool ?P then _ else _] => destruct P; [tauto|simpl; rewrite wzero_wor]
           end.
           match goal with
-          | |- context [wnot ?P] => rewrite <- (natToWord_wordToNat (wnot P))
+          | |- context [wnot _ ?P] => rewrite <- (natToWord_wordToNat _ (wnot _ P))
           end.
           rewrite ?wordToNat_wnot.
           match goal with
-          | |- context [combine ?P ?Q] => (rewrite <- (natToWord_wordToNat (combine P Q)))
+          | |- context [wconcat ?P ?Q] => (rewrite <- (natToWord_wordToNat _ (wconcat P Q)))
           end.
           rewrite ?wordToNat_combine; simpl.
           rewrite ?Nat.mul_1_r, ?Nat.mul_0_r, ?Nat.add_0_r.
           rewrite wordToNat_natToWord_idempotent'.
           * rewrite <- ?natToWord_plus.
             match goal with
-            | |- context[?A - #(?B) - 1 + (2 + ?P)] => pose proof (wordToNat_bound B) as sth0;
-                                                         assert (sth1: A > #B) by lia;
-                                                         assert (sth2: A - #B - 1 + (2 + P) = A + P + 1 - #B) by lia; rewrite ?sth2;
+            | |- context[?A - wordToNat _ (?B) - 1 + (2 + ?P)] => pose proof (wordToNat_bound B) as sth0;
+                                                         assert (sth1: A > wordToNat _ B) by lia;
+                                                         assert (sth2: A - wordToNat _ B - 1 + (2 + P) = A + P + 1 - wordToNat _ B) by lia; rewrite ?sth2;
                                                            remember B as val
             end.
             Transparent normDist.
             unfold normDist in Heqval.
             simpl in Heqval.
             match goal with
-            | [H: val = if getBool (weq ?w1 ?w2) then _ else _ |- _] => destruct (weq w1 w2); simpl in *
+            | [H: val = if getBool (weq _ ?w1 ?w2) then _ else _ |- _] => destruct (weq _ w1 w2); simpl in *
             end.
             ***
                subst.
-               assert (sth3: pow2 (expWidth + 1) + pow2 expWidthMinus1 + 1 - sigWidthMinus2 = pow2 (expWidth + 1) + (pow2 expWidthMinus1 + 1 - sigWidthMinus2)). {
+               assert (sth3: 2 ^ (expWidth + 1) + 2 ^ expWidthMinus1 + 1 - sigWidthMinus2 = 2 ^ (expWidth + 1) + (2 ^ expWidthMinus1 + 1 - sigWidthMinus2)). {
                  pose proof expWidth_ge_sigWidth.
                  rewrite Nat.add_sub_assoc; lia.
                }
-               assert (sigWidthMinus2 < pow2 (expWidth + 1)). {
+               assert (sigWidthMinus2 < 2 ^ (expWidth + 1)). {
                  rewrite ?Nat.pow_add_r; simpl.
                  rewrite ?Nat.pow_add_r; simpl.
                  pose proof (pow2_zero expWidthMinus2).
@@ -590,9 +611,9 @@ Section Properties.
                split; auto.
                lia.
                pose proof expWidth_ge_sigWidth.
-               apply lt_minus; lia.
+               apply lt_minus'; lia.
                pose proof expWidth_ge_sigWidth.
-               apply lt_minus. lia.
+               apply lt_minus'. lia.
                rewrite Nat.add_1_r.
                simpl; lia.
                rewrite ?Nat.add_1_r.
@@ -601,7 +622,7 @@ Section Properties.
                apply Plus.plus_lt_compat_l.
                rewrite ?Nat.add_0_r.
                rewrite <- mul2_add. 
-               replace (pow2 expWidthMinus2 * 2) with (pow2 expWidthMinus2 * pow2 1) by (simpl;reflexivity).
+               replace (2 ^ expWidthMinus2 * 2) with (2 ^ expWidthMinus2 * 2 ^ 1) by (simpl;reflexivity).
                rewrite <- Nat.pow_add_r.
                lia.
 
@@ -615,12 +636,12 @@ Section Properties.
                rewrite wzero_wplus.
                rewrite split1_fits_natToWord.
                rewrite Nat.add_1_r.
-               assert (sth4: pow2 (S expWidthMinus2) + 1 - sigWidthMinus2 < 2 * pow2 expWidthMinus2). { 
+               assert (sth4: 2 ^ (S expWidthMinus2) + 1 - sigWidthMinus2 < 2 * 2 ^ expWidthMinus2). { 
                  rewrite Nat.add_comm.
                  rewrite <- Nat.add_sub_assoc.
                  rewrite Nat.add_comm.
-                 assert (sth4: 2 * pow2 expWidthMinus2 = pow2 (S expWidthMinus2)). {
-                   assert (pow2 1 = 2). auto.
+                 assert (sth4: 2 * 2 ^ expWidthMinus2 = 2 ^ (S expWidthMinus2)). {
+                   assert (2 ^ 1 = 2). auto.
                    rewrite <- H2 at 1.
                    rewrite <- pow2_add_mul.
                    rewrite <- Nat.add_1_r. auto.
@@ -630,7 +651,7 @@ Section Properties.
                  rewrite sth4.
                  replace (S (S sigWidthMinus4)) with (sigWidthMinus4 + 1 + 1) by lia.
                  rewrite Nat.sub_add_distr.
-                 replace (pow2 (S expWidthMinus2) - (sigWidthMinus4 + 1) - 1 + 1) with (pow2 (S expWidthMinus2) - (sigWidthMinus4 + 1)) by lia. 
+                 replace (2 ^ (S expWidthMinus2) - (sigWidthMinus4 + 1) - 1 + 1) with (2 ^ (S expWidthMinus2) - (sigWidthMinus4 + 1)) by lia. 
                  rewrite <- Heq in *.
                  pose proof expWidth_ge_sigWidth.
                  apply Nat.sub_lt; lia.
@@ -643,9 +664,9 @@ Section Properties.
                split; auto.
                simpl.
                assert (sth5: 
-                         pow2 expWidthMinus2 + (pow2 expWidthMinus2 + 0) + 1 - sigWidthMinus2 =
+                         2 ^ expWidthMinus2 + (2 ^ expWidthMinus2 + 0) + 1 - sigWidthMinus2 =
                          
-                         pow2 expWidthMinus2 + ((pow2 expWidthMinus2 + 0) + 1 - sigWidthMinus2)). {
+                         2 ^ expWidthMinus2 + ((2 ^ expWidthMinus2 + 0) + 1 - sigWidthMinus2)). {
                  pose proof expWidth_ge_sigWidth.
                  rewrite Nat.add_sub_assoc; lia.
                }
@@ -653,7 +674,7 @@ Section Properties.
                rewrite <- Nat.add_0_r at 1.
                apply Plus.plus_le_compat_l.
                lia.
-               apply lt_minus; try lia.
+               apply lt_minus'; try lia.
                rewrite Nat.add_1_r.
                simpl.
                rewrite ?Nat.add_1_r.
@@ -664,7 +685,7 @@ Section Properties.
                lia.
             *** rewrite evalExpr_countLeadingZeros in Heqval.
             pose proof expWidth_ge_sigWidth as sth3.
-            assert (sth4: pow2 (expWidth + 1) > sigWidthMinus1). {
+            assert (sth4: 2 ^ (expWidth + 1) > sigWidthMinus1). {
               rewrite ?Nat.pow_add_r; simpl.
               pose proof (pow2_zero expWidthMinus2).
               nia.
@@ -676,28 +697,28 @@ Section Properties.
             | getBool ?P = false => destruct P; [discriminate|]
             end.
             match type of Heqval with
-            | _ = countLeadingZerosWord _ ?P =>
+            | _ = countLeadingZerosWord _ _ ?P =>
               pose proof (countLeadingZerosWord_lt_len _ sth4 n0) as sth5
             end.
             rewrite <- Heqval in sth5.
             apply wordToNat_lt1 in sth5.
             rewrite wordToNat_natToWord_idempotent' in sth5 by assumption.
-            assert (sth6: pow2 (expWidth + 1) + pow2 expWidthMinus1 + 1 - #val >= pow2 (expWidth + 1) + pow2 expWidthMinus1 - pow2 expWidthMinus2) by lia.
-            remember (pow2 (expWidth + 1) + pow2 expWidthMinus1 + 1 - #val) as val2.
+            assert (sth6: 2 ^ (expWidth + 1) + 2 ^ expWidthMinus1 + 1 - wordToNat _ val >= 2 ^ (expWidth + 1) + 2 ^ expWidthMinus1 - 2 ^ expWidthMinus2) by lia.
+            remember (2 ^ (expWidth + 1) + 2 ^ expWidthMinus1 + 1 - wordToNat _ val) as val2.
             repeat match goal with
-                   | |- context[weq (split2 ?A ?B ?P) _] =>
-                     rewrite <- (natToWord_wordToNat (split2 A B P))
-                   | |- context[weq (split1 ?A ?B ?P) _] =>
-                     rewrite <- (natToWord_wordToNat (split1 A B P))
+                   | |- context[weq _ (@truncMsb ?A ?B ?P) _] =>
+                     rewrite <- (natToWord_wordToNat _ (@truncMsb A B P))
+                   | |- context[weq _ (@truncLsb ?A ?B ?P) _] =>
+                     rewrite <- (natToWord_wordToNat _ (@truncLsb A B P))
                    end.
-            assert (sth7: val2 <= pow2 (expWidth + 1) + pow2 expWidthMinus1 + 1) by lia.
+            assert (sth7: val2 <= 2 ^ (expWidth + 1) + 2 ^ expWidthMinus1 + 1) by lia.
             rewrite ?wordToNat_split2, ?wordToNat_split1.
             rewrite mod_factor' with (c := 2).
             -- rewrite <- andb_assoc.
                rewrite andb_false_iff; right.
-               assert (sth8: val2 >= pow2 (expWidth + 1)) by lia.
-               assert (sth9: val2 >= 2 * pow2 expWidth) by (rewrite Nat.pow_add_r in sth8; simpl in sth8; nia).
-               assert (sth10: val2 >= 4 * pow2 (expWidthMinus1)) by (do 2 (rewrite Nat.pow_add_r in sth8); simpl in sth8; nia).
+               assert (sth8: val2 >= 2 ^ (expWidth + 1)) by lia.
+               assert (sth9: val2 >= 2 * 2 ^ expWidth) by (rewrite Nat.pow_add_r in sth8; simpl in sth8; nia).
+               assert (sth10: val2 >= 4 * 2 ^ (expWidthMinus1)) by (do 2 (rewrite Nat.pow_add_r in sth8); simpl in sth8; nia).
                rewrite ?wordToNat_natToWord_eqn.
                rewrite mod_factor' with (c := 2) by (pose proof (pow2_zero expWidth); try lia; rewrite ?Nat.pow_add_r; auto).
                rewrite mod_factor' with (c := (2 * 2)).
@@ -706,11 +727,11 @@ Section Properties.
                   rewrite <- mod_sub with (b := 2) by auto. 
                   rewrite <- mod_sub with (a := val2) (b := 4) by auto.
                   rewrite Nat.mod_small.
-                  ** assert (sth13: pow2 expWidthMinus1 - pow2 expWidthMinus2 <= val2 - pow2 (expWidth + 1) <= pow2 expWidthMinus1 + 1) by lia.
-                     destruct (Compare_dec.le_lt_dec (val2 - pow2 (expWidth + 1)) (pow2 expWidthMinus1 - 1)).
+                  ** assert (sth13: 2 ^ expWidthMinus1 - 2 ^ expWidthMinus2 <= val2 - 2 ^ (expWidth + 1) <= 2 ^ expWidthMinus1 + 1) by lia.
+                     destruct (Compare_dec.le_lt_dec (val2 - 2 ^ (expWidth + 1)) (2 ^ expWidthMinus1 - 1)).
                      --- rewrite andb_false_iff; right.
                          rewrite Nat.mod_small.
-                         +++ assert (th0: pow2 (expWidth + 1) = 4 * pow2 expWidthMinus1). {
+                         +++ assert (th0: 2 ^ (expWidth + 1) = 4 * 2 ^ expWidthMinus1). {
                                rewrite Nat.pow_add_r with (b := expWidth).
                                rewrite Nat.pow_add_r with (b := expWidthMinus1).
                                clear.
@@ -718,30 +739,30 @@ Section Properties.
                                lia.
                              }
                              rewrite <- th0.
-                             remember (val2 - pow2 (expWidth + 1)) as val3.
-                             assert (th01: pow2 expWidthMinus1 = pow2 expWidthMinus2 * 2) by (rewrite Nat.pow_add_r; auto).
+                             remember (val2 - 2 ^ (expWidth + 1)) as val3.
+                             assert (th01: 2 ^ expWidthMinus1 = 2 ^ expWidthMinus2 * 2) by (rewrite Nat.pow_add_r; auto).
                              rewrite th01 in *.
-                             assert (th1: val3 < pow2 expWidthMinus2 * 2) by lia.
-                             assert (th2: val3 >= pow2 expWidthMinus2 * 1) by lia.
-                             assert (th3: pow2 expWidthMinus2 <> 0) by (clear; pose proof (pow2_zero expWidthMinus2); lia).
+                             assert (th1: val3 < 2 ^ expWidthMinus2 * 2) by lia.
+                             assert (th2: val3 >= 2 ^ expWidthMinus2 * 1) by lia.
+                             assert (th3: 2 ^ expWidthMinus2 <> 0) by (clear; pose proof (pow2_zero expWidthMinus2); lia).
                              pose proof (Nat.div_lt_upper_bound _ _ _ th3 th1) as th4.
                              pose proof (Nat.div_le_lower_bound _ _ _ th3 th2) as th5.
-                             assert (th6: val3 / pow2 expWidthMinus2 = 1) by (clear - th4 th5; lia).
+                             assert (th6: val3 / 2 ^ expWidthMinus2 = 1) by (clear - th4 th5; lia).
                              rewrite th6; auto.
                          +++ clear - l.
                              rewrite Nat.pow_add_r with (b := expWidth) in l; simpl in l.
                              rewrite Nat.pow_add_r with (b := expWidthMinus1) in l; simpl in l.
                              pose proof (pow2_zero expWidthMinus1); lia.
-                     --- assert (sth14: pow2 (expWidth + 1) = 2 * pow2 expWidth) by
+                     --- assert (sth14: 2 ^ (expWidth + 1) = 2 * 2 ^ expWidth) by
                            (clear; rewrite Nat.pow_add_r; simpl; lia).
                          rewrite <- sth14.
-                         remember (val2 - pow2 (expWidth + 1)) as val3.
-                         assert (th1: val3 < pow2 expWidthMinus1 * 2) by lia.
-                         assert (th2: val3 >= pow2 expWidthMinus1 * 1) by lia.
-                         assert (th3: pow2 expWidthMinus1 <> 0) by (clear - sth12; lia).
+                         remember (val2 - 2 ^ (expWidth + 1)) as val3.
+                         assert (th1: val3 < 2 ^ expWidthMinus1 * 2) by lia.
+                         assert (th2: val3 >= 2 ^ expWidthMinus1 * 1) by lia.
+                         assert (th3: 2 ^ expWidthMinus1 <> 0) by (clear - sth12; lia).
                          pose proof (Nat.div_lt_upper_bound _ _ _ th3 th1) as th4.
                          pose proof (Nat.div_le_lower_bound _ _ _ th3 th2) as th5.
-                         assert (th6: val3 / pow2 expWidthMinus1 = 1) by (clear - th4 th5; lia).
+                         assert (th6: val3 / 2 ^ expWidthMinus1 = 1) by (clear - th4 th5; lia).
                          rewrite th6; auto.
                   ** clear - sth7.
                      rewrite ?Nat.pow_add_r in *; simpl in *.
@@ -759,14 +780,17 @@ Section Properties.
             destruct expWidthMinus2; simpl; try lia.
             pose proof (pow2_zero n0).
             lia.
+          * auto.
+          * auto.
+          * auto.
         + rewrite ?wzero_wplus.
           rewrite ?split1_combine_wplus.
           rewrite andb_false_iff.
           left.
           match goal with
-          | |- getBool (weq ?P _) && getBool (weq ?Q _) = _ =>
-            rewrite <- (natToWord_wordToNat P);
-              rewrite <- (natToWord_wordToNat Q)
+          | |- getBool (weq _ ?P _) && getBool (weq _ ?Q _) = _ =>
+            rewrite <- (natToWord_wordToNat _ P);
+              rewrite <- (natToWord_wordToNat _ Q)
           end.
           rewrite ?wordToNat_split2.
           rewrite ?wordToNat_wplus, ?wordToNat_combine; simpl.
@@ -774,18 +798,18 @@ Section Properties.
           rewrite wordToNat_natToWord_idempotent' by
               (rewrite ?Nat.pow_add_r; simpl; pose proof (pow2_zero expWidthMinus2); lia).
           simpl.
-          rewrite Nat.mod_small with (b := pow2 (expWidth + 1)); simpl.
+          rewrite Nat.mod_small with (b := 2 ^ (expWidth + 1)); simpl.
           * match goal with
-              |- context [#(?A)] => remember A as val; simpl in *
+              |- context [wordToNat _ (?A)] => remember A as val; simpl in *
             end.
-            assert (sth: #val + S (pow2 expWidthMinus1) < pow2 expWidth * 2). {
+            assert (sth: wordToNat _ val + S (2 ^ expWidthMinus1) < 2 ^ expWidth * 2). {
               pose proof (wordToNat_bound val).
               rewrite ?Nat.pow_add_r with (b := expWidthMinus1) in *; simpl in *.
               pose proof (pow2_zero expWidthMinus1).
               nia.
             }
             pose proof (pow2_zero expWidth) as sth2.
-            pose proof (Nat.div_lt_upper_bound _ (pow2 expWidth) 2 ltac:(lia) sth) as sth3.
+            pose proof (Nat.div_lt_upper_bound _ (2 ^ expWidth) 2 ltac:(lia) sth) as sth3.
             simpl in sth3.
             match type of sth3 with
             | ?P < 2 => case_eq P; intros
@@ -793,15 +817,15 @@ Section Properties.
             -- simpl.
                rewrite Nat.div_small_iff in H0 by (pose proof (pow2_zero expWidth); lia).
                rewrite Nat.mod_small by assumption.
-               assert (sth4: pow2 expWidthMinus1 * 1 <= #val + S (pow2 expWidthMinus1)) by lia.
+               assert (sth4: 2 ^ expWidthMinus1 * 1 <= wordToNat _ val + S (2 ^ expWidthMinus1)) by lia.
                simpl in *.
                pose proof (pow2_zero expWidthMinus1) as sth5.
-               pose proof (Nat.div_le_lower_bound _ (pow2 expWidthMinus1) 1 ltac:(lia) sth4) as sth6.
+               pose proof (Nat.div_le_lower_bound _ (2 ^ expWidthMinus1) 1 ltac:(lia) sth4) as sth6.
                assert (sth7:
-                         #val + S (pow2 expWidthMinus1) < pow2 expWidthMinus1 * 2) by
+                         wordToNat _ val + S (2 ^ expWidthMinus1) < 2 ^ expWidthMinus1 * 2) by
                    (rewrite Nat.pow_add_r with (b := expWidthMinus1) in H0; simpl in *; assumption).
                simpl in *.
-               pose proof (Nat.div_lt_upper_bound _ (pow2 expWidthMinus1) 2 ltac:(lia) sth7) as
+               pose proof (Nat.div_lt_upper_bound _ (2 ^ expWidthMinus1) 2 ltac:(lia) sth7) as
                    sth8.
                match goal with
                | |- context [(?P + ?Q)/?R] => destruct ((P + Q)/R); simpl; try lia
@@ -809,11 +833,15 @@ Section Properties.
                destruct n; auto; lia.
             -- destruct n; [auto|lia].
           * match goal with
-            | |- #(?P) + _ < _ => pose proof (wordToNat_bound P)
+            | |- wordToNat _ ?P + _ < _ => pose proof (wordToNat_bound P)
             end.
             rewrite ?Nat.pow_add_r in *; simpl in *.
             pose proof (pow2_zero expWidthMinus2).
             nia.
+          * auto.
+          * auto.
+          * auto.
+          * auto.
             Transparent isNaN_or_Inf infOrNaN isZeroFractIn isSpecial normDist subnormFract isZeroExpIn.
     Qed.
 
@@ -854,6 +882,7 @@ Section Properties.
       unfold natToWord; simpl.
       pose proof (infOrNaN_isZeroNaNInf2_1_isZeroFractIn H) as sth.
       simpl in sth.
+      assert (sth' : ZToWord 1 1 = natToWord 1 1) by auto. rewrite sth'. clear sth'.
       rewrite sth.
       f_equal.
       case_eq (evalExpr (isZeroExpIn fn)); auto; intros.
@@ -869,15 +898,6 @@ Section Properties.
       apply getBool_weq in H0.
       pose proof (@wzero_wones expWidth ltac:(lia)).
       congruence.
-    Qed.
-
-    Lemma if_bool_2 A (x y: A) (p1 p2: bool):
-      p1 = p2 ->
-      (if p1 then x else y) = (if p2 then x else y).
-    Proof.
-      intros sth.
-      rewrite sth.
-      auto.
     Qed.
 
     Lemma bool_prop2 a b c:
@@ -912,7 +932,7 @@ Section Properties.
           Transparent isNaN_or_Inf infOrNaN isZeroNaNInf2 isZeroFractIn isSpecial normDist subnormFract isZeroExpIn isZeroRecFN isSigNaNRawFloat
                       isSigNaNRawFloat_frac isSNaN.
     Qed.
-    
+
     Lemma get_exp_from_RecFN_adjustedExp:
       evalExpr (isFiniteNonzero (getRawFloat_from_FN fn)) = true ->
       evalExpr (get_exp_from_RecFN (getRecFN_from_FN fn)) = evalExpr (adjustedExp fn).
@@ -923,6 +943,7 @@ Section Properties.
       intros.
       repeat (rewrite andb_true_iff in *; dest).
       repeat rewrite negb_true_iff in *.
+      rewrite !wconcat_w_0.
       rewrite ?split1_combine, ?split2_combine.
       rewrite ?wzero_wplus, ?wor_wzero, ?wzero_wor.
       rewrite isSpecial_infOrNaN in *.
@@ -932,9 +953,9 @@ Section Properties.
       - rewrite H0 in *; simpl in *.
         rewrite andb_true_r in *.
         rewrite H.
-        rewrite ?wor_wzer, ?wzero_wor.
-        rewrite ?combine_split.
-        auto.
+        rewrite ?wor_wzero, ?wzero_wor.
+        rewrite ?concat_split'.
+        auto. 
       - assert (sth2: evalExpr (infOrNaN fn) = false). {
           match type of H1 with
           | _ && ?P = false => destruct P; auto; simpl in *
@@ -944,8 +965,8 @@ Section Properties.
         }
         rewrite sth2 in *; simpl in *.
         rewrite ?wor_wzer, ?wzero_wor.
-        rewrite ?combine_split.
-        auto.
+        rewrite ?concat_split'.
+        auto. 
         Transparent isNaN_or_Inf infOrNaN isZeroFractIn isSpecial normDist subnormFract isZeroExpIn isZeroRecFN isSigNaNRawFloat
                     isSigNaNRawFloat_frac isSNaN.
     Qed.
@@ -966,6 +987,8 @@ Section Properties.
                   isSigNaNRawFloat_frac isSNaN sExp_expWidth sExp_expWidthMinus1 sExp_expWidthMinus2 isZeroNaNInf1 isZeroNaNInf0 get_exp_from_RecFN adjustedExp.
     Qed.
 
+    Print wltu.
+
     Lemma isSubnormal_isZeroExpIn_simple:
       evalExpr (isFiniteNonzero (getRawFloat_from_FN fn)) = true ->
       evalExpr (isSubnormal (getRawFloat_from_FN fn)) = evalExpr (isZeroExpIn fn).
@@ -974,38 +997,41 @@ Section Properties.
       Opaque isNaN_or_Inf infOrNaN isZeroNaNInf2 isZeroFractIn isSpecial normDist subnormFract isZeroExpIn isZero isZeroRecFN isSigNaNRawFloat
              isSigNaNRawFloat_frac isSNaN get_exp_from_RecFN.
       simpl.
+      rewrite wconcat_w_0.
       rewrite wzero_wplus.
       rewrite ?split2_combine.
       simpl.
-      unfold wzero; simpl.
       unfold natToWord; fold natToWord.
       simpl.
       case_eq (evalExpr (isZeroExpIn fn)); intros sth.
-      - match goal with
+      - rewrite wltu_wordToNat.
+        apply Nat.ltb_lt.
+        (* match goal with
         | |- getBool ?P = true => destruct P; simpl; auto
         end.
-        pre_word_omega.
-        rewrite ?wordToNat_combine in *; simpl in *; rewrite ?Nat.mul_0_r, ?Nat.mul_1_r, ?Nat.add_0_r in *.
+        pre_word_omega. *)
+        rewrite ?wordToNat_combine in *; auto; simpl in *; rewrite ?Nat.mul_0_r, ?Nat.mul_1_r, ?Nat.add_0_r in *.
         rewrite wordToNat_wplus in *.
-        rewrite ?wordToNat_combine in *; simpl in *; rewrite ?Nat.mul_0_r, ?Nat.mul_1_r, ?Nat.add_0_r in *.
+        rewrite ?wordToNat_combine in *; auto; simpl in *; rewrite ?Nat.mul_0_r, ?Nat.mul_1_r, ?Nat.add_0_r in *.
         rewrite wordToNat_wnot in *; simpl in *.
+        replace (ZToWord _ 2) with (natToWord expWidthMinus1 2); auto.
         rewrite wordToNat_natToWord_idempotent' in *.
-        + assert (sth0: pow2 (expWidth + 1) >= # (evalExpr (normDist fn))). {
+        + assert (sth0: 2 ^ (expWidth + 1) >= wordToNat _ (evalExpr (normDist fn))). {
             pose proof (wordToNat_bound (evalExpr (normDist fn))) as sth2.
             simpl in sth2.
             lia.
           }
-          assert (sth1: pow2 (expWidth + 1) >= # (evalExpr (normDist fn)) + 1). {
+          assert (sth1: 2 ^ (expWidth + 1) >= wordToNat _ (evalExpr (normDist fn)) + 1). {
             pose proof (wordToNat_bound (evalExpr (normDist fn))) as sth2.
             simpl in sth2.
             lia.
           }
-          assert (sth2: sigWidthMinus1 < pow2 (expWidth + 1)). {
+          assert (sth2: sigWidthMinus1 < 2 ^ (expWidth + 1)). {
             pose proof expWidth_ge_sigWidth.
             do 2 (rewrite Nat.pow_add_r; simpl).
             lia.
           }
-          assert (sth3: 2 + pow2 expWidthMinus1 >= #(evalExpr (normDist fn)) + 1). {
+          assert (sth3: 2 + 2 ^ expWidthMinus1 >=  wordToNat _ (evalExpr (normDist fn)) + 1). {
             Transparent normDist.
             unfold normDist; simpl.
             match goal with
@@ -1017,51 +1043,57 @@ Section Properties.
             lia.
             rewrite evalExpr_countLeadingZeros; simpl.
             match goal with
-            | |- _ >= #(countLeadingZerosWord _ ?P) + 1 =>
+            | |- _ >= wordToNat _ (countLeadingZerosWord _ _ ?P) + 1 =>
               remember P as val;
-                pose proof (countLeadingZerosWord_le_len sth2 val); simpl in *
+                pose proof (countLeadingZerosWord_le_len _ sth2 val); simpl in *
             end.
-            pre_word_omega.
+            rewrite wleu_wordToNat in H. apply Nat.leb_le in H.
             rewrite wordToNat_natToWord_idempotent' in H by assumption.
-            assert (sth15: pow2 expWidthMinus2 + 4 >= #(countLeadingZerosWord (expWidth + 1) val) + 1) by lia.
-            assert (sth25: pow2 expWidthMinus2 + 4 <= S (S (pow2 expWidthMinus1))). {
+            assert (sth15: 2 ^ expWidthMinus2 + 4 >= wordToNat _ (countLeadingZerosWord _ (expWidth + 1) val) + 1) by lia.
+            assert (sth25: 2 ^ expWidthMinus2 + 4 <= S (S (2 ^ expWidthMinus1))). {
               rewrite Nat.pow_add_r; simpl.
-              assert (pow2 expWidthMinus2 >= 2). {
+              assert (2 ^ expWidthMinus2 >= 2). {
                 destruct expWidthMinus2; try lia.
-                destruct n1; try lia.
+                destruct n0; try lia.
                 simpl.
-                pose proof (pow2_zero n1); lia.
+                pose proof (pow2_zero n0); lia.
               }
               lia.
             }
             lia.
           }
-          assert (sth4: pow2 (expWidth + 1) - # (evalExpr (normDist fn)) - 1 +
-                        (2 + pow2 expWidthMinus1)
-                        = ((2 + pow2 expWidthMinus1) - (#(evalExpr (normDist fn)) + 1)) + 1 * pow2 (expWidth + 1)) by lia.
+          assert (sth4: 2 ^ (expWidth + 1) - wordToNat _ (evalExpr (normDist fn)) - 1 +
+                        (2 + 2 ^ expWidthMinus1)
+                        = ((2 + 2 ^ expWidthMinus1) - (wordToNat _ (evalExpr (normDist fn)) + 1)) + 1 * 2 ^ (expWidth + 1)) by lia.
           rewrite sth4 in *.
-          rewrite Nat.mod_add in n by (pose proof (pow2_zero (expWidth + 1)); lia).
-          rewrite Nat.mod_small in n.
+          rewrite Nat.mod_add by (pose proof (pow2_zero (expWidth + 1)); lia).
+          rewrite Nat.mod_small.
           * lia.
           * pose proof (pow2_zero expWidthMinus2).
             rewrite ?Nat.pow_add_r; simpl.
             match goal with
             | |- match ?P with _ => _ end < _ => destruct P; try lia
             end.
-            destruct n0; try lia.
+            destruct n; try lia.
         + rewrite ?Nat.pow_add_r in *; simpl.
           destruct expWidthMinus2; try lia; simpl.
-          pose proof (pow2_zero n0); lia.
-      - match goal with
-        | |- getBool ?P = false => destruct P; simpl; auto
-        end.
-        pre_word_omega.
-        rewrite wordToNat_combine in w; simpl in *; rewrite Nat.mul_0_r, Nat.add_0_r in *.
+          pose proof (pow2_zero n); lia.
+      - rewrite wconcat_w_0.
+        rewrite wltu_wordToNat.
+        apply Nat.ltb_nlt.
+        (* pre_word_omega. *)
+        rewrite wordToNat_combine; auto; simpl in *.
+        replace (wordToNat 1 WO~0) with 0; auto.
+        rewrite Nat.mul_0_r, Nat.add_0_r in *.
         rewrite wordToNat_wplus in *.
-        rewrite ?wordToNat_combine in w; simpl in *; rewrite Nat.mul_0_r, Nat.mul_1_r, ?Nat.add_0_r in *.
+        rewrite ?wordToNat_combine; auto; simpl in *.
+        replace (wordToNat 1 WO~0) with 0; auto.
+        rewrite Nat.mul_0_r, Nat.mul_1_r, ?Nat.add_0_r in *.
+        replace (ZToWord _ 1) with (natToWord expWidthMinus1 1); auto.
+        replace (ZToWord _ 2) with (natToWord expWidthMinus1 2); auto.
         rewrite wordToNat_natToWord_idempotent' in * by (rewrite Nat.pow_add_r; simpl; pose proof (pow2_zero expWidthMinus2); lia).
         rewrite ?Nat.mul_0_r, ?Nat.mul_1_r, ?Nat.add_0_r in *.
-        rewrite wordToNat_natToWord_idempotent' in * at 2.
+        rewrite wordToNat_natToWord_idempotent' in *.
         + rewrite Nat.mod_small in *.
           * Transparent isZeroExpIn.
             unfold isZeroExpIn in *; simpl in *.
@@ -1072,7 +1104,7 @@ Section Properties.
             lia.
             Opaque isZeroExpIn.
           * match goal with
-            | |- #?a + _ < _ => pose proof (wordToNat_bound a) as sth1
+            | |- wordToNat _ ?a + _ < _ => pose proof (wordToNat_bound a) as sth1
             end.
             rewrite ?Nat.pow_add_r in *; simpl in *.
             pose proof (pow2_zero expWidthMinus2) as sth2.
@@ -1082,7 +1114,7 @@ Section Properties.
           destruct expWidthMinus2; simpl; try lia.
           pose proof pow2_zero n; lia.
       Transparent isNaN_or_Inf infOrNaN isZeroNaNInf2 isZeroFractIn isSpecial normDist subnormFract isZeroExpIn isZero isZeroRecFN isSigNaNRawFloat
-             isSigNaNRawFloat_frac isSNaN get_exp_from_RecFN.
+             isSigNaNRawFloat_frac isSNaN get_exp_from_RecFN. 
     Qed.
     
     Lemma isSubnormal_isZeroExpIn_complex:
@@ -1127,7 +1159,7 @@ Section Properties.
                   isSigNaNRawFloat_frac isSNaN.
     Qed.
         
-    Lemma sigWidthMinus1_lt_pow2_expWidth: (sigWidthMinus1 < pow2 expWidth).
+    Lemma sigWidthMinus1_lt_pow2_expWidth: (sigWidthMinus1 < 2 ^ expWidth).
     Proof.
       rewrite ?Nat.pow_add_r.
       simpl. 
@@ -1136,7 +1168,7 @@ Section Properties.
     Qed.
 
     Lemma expWidthMinus2_le_expWidth_plus1:
-      pow2 expWidthMinus2 + 4 < pow2 (expWidth + 1).
+      2 ^ expWidthMinus2 + 4 < 2 ^ (expWidth + 1).
     Proof.
       clear fn expWidthMinus2_plus4_gt_sigWidth expWidth_prop.
       induction expWidthMinus2; simpl; auto.
@@ -1144,7 +1176,7 @@ Section Properties.
     Qed.
 
     Lemma expWidthMinus2_le_expWidth:
-      pow2 expWidthMinus2 + 4 < pow2 expWidth.
+      2 ^ expWidthMinus2 + 4 < 2 ^ expWidth.
     Proof.
       clear fn expWidthMinus2_plus4_gt_sigWidth.
       induction expWidthMinus2.
@@ -1154,71 +1186,8 @@ Section Properties.
         destruct sth as [sth1|sth1]; try rewrite sth1; simpl in *; lia.
     Qed.
         
-    Lemma mod_cancel_l:
-      forall a b x n,
-        n <> 0 ->
-        a mod n = b mod n ->
-        (x + a) mod n = (x + b) mod n.
-    Proof.
-      intros.
-      rewrite <- Nat.add_mod_idemp_r; auto.
-      rewrite H0.
-      rewrite Nat.add_mod_idemp_r; auto.
-    Qed.
-    
-    Lemma pow2_1_iff_0 n:
-      pow2 n = 1 <-> n = 0.
-    Proof.
-      induction n; split; intro; try lia.
-      simpl. reflexivity.
-      destruct IHn.
-      pose proof (one_lt_pow2 n) as sth1.
-      rewrite H in sth1.
-      apply False_ind.
-      inversion sth1.
-      inversion H3.
-    Qed.
-      
-    Lemma pow2_lt_S n:
-      n > 0 ->
-      pow2 n + 1 < pow2 (n + 1).
-    Proof.
-      pose proof (pow2_le_S n) as sth.
-      apply Nat.lt_eq_cases in sth.
-      destruct sth; auto.
-      intro sth.
-      apply False_ind.
-      apply Nat.add_sub_eq_l in H.
-      pose proof (pow2_1_iff_0 n) as sth1.
-      replace (pow2 n) with (pow2 n * 1) in H by lia.
-      rewrite pow2_add_mul in H.
-      rewrite <- Nat.mul_sub_distr_l in H.
-      simpl in H.
-      destruct sth1 as [sth2 sth3].
-      rewrite sth2 in sth; lia.
-    Qed.
-
-    Lemma pow2_lt_2 n:
-      1 < n -> 2 < pow2 n.
-    Proof.
-      intro sth.
-      induction n.
-      inversion sth.
-      simpl.
-      assert (sth1: n = 1 \/ n > 1) by lia.
-      destruct sth1.
-      rewrite H.
-      simpl.
-      auto.
-      simpl.
-      apply Nat.lt_lt_add_l.
-      rewrite Nat.add_0_r.
-      lia.
-    Qed.
-
-
     Lemma normalizedExp_adjustedExp:
-      evalExpr (normalizedExp fn) = evalExpr (adjustedExp fn + $ (pow2 expWidth))%kami_expr.
+      evalExpr (normalizedExp fn) = evalExpr (adjustedExp fn + $ (2 ^ expWidth))%kami_expr.
     Proof.
       unfold normalizedExp, adjustedExp.
       Opaque isZeroExpIn normDist.
@@ -1226,7 +1195,7 @@ Section Properties.
       pose proof (@pow2_lt_2 expWidthMinus1 ltac:(lia)) as sth.
       pose proof (@pow2_lt_2 expWidth ltac:(lia)) as sth1.
       pose proof (pow2_lt_pow2_S expWidthMinus1) as sth2.
-      assert (sth3: pow2 expWidthMinus1 * 2 = pow2 expWidth). {
+      assert (sth3: 2 ^ expWidthMinus1 * 2 = 2 ^ expWidth). {
         rewrite (Nat.add_1_r expWidthMinus1).
         simpl.
         lia.
@@ -1247,6 +1216,7 @@ Section Properties.
         rewrite <- ?wplus_assoc.
         apply word_cancel_l.
         apply word_cancel_l.
+        rewrite wconcat_w_0.
         rewrite combine_shiftl_plus_n; auto.
         rewrite combine_wplus.
         simpl.
@@ -1257,11 +1227,11 @@ Section Properties.
         rewrite <- wplus_assoc.
         apply word_cancel_l.
         rewrite wplus_comm.
-        apply move_wplus_wminus.
+        apply move_wplus_wminus'.
         rewrite wminus_def.
         symmetry.
         rewrite wplus_comm.
-        apply move_wplus_wminus.
+        apply move_wplus_wminus'.
         rewrite wminus_def.
         rewrite wneg_idempotent.
         rewrite <- natToWord_plus.
@@ -1274,30 +1244,31 @@ Section Properties.
         rewrite Nat.add_1_r.
         simpl.
         lia.
-      + rewrite wminus_simple_wminus.
+      + (* rewrite wminus_simple_wminus. *)
         rewrite ?wzero_wplus. 
         rewrite ?wminus_def.
         rewrite <- wplus_assoc.
         apply word_cancel_l.
+        rewrite wconcat_w_0.
         rewrite combine_shiftl_plus_n; [| intuition].
         rewrite <- natToWord_plus.
         rewrite combine_natToWord_wzero; [ |lia].
         symmetry.
-        apply move_wplus_wminus.
+        apply move_wplus_wminus'.
         rewrite wminus_def.
         rewrite wplus_comm.
         symmetry.
-        apply move_wplus_wminus.
+        apply move_wplus_wminus'.
         rewrite wminus_def.
         rewrite wneg_idempotent.
         rewrite <- natToWord_plus.
-        replace (pow2 expWidthMinus1 + 1 + (pow2 expWidthMinus1 - 1)) with
-            (pow2 expWidthMinus1 + pow2 expWidthMinus1) by lia.
+        replace (2 ^ expWidthMinus1 + 1 + (2 ^ expWidthMinus1 - 1)) with
+            (2 ^ expWidthMinus1 + 2 ^ expWidthMinus1) by lia.
         rewrite <- mul2_add.
         rewrite sth3.
         rewrite Nat.add_1_r.
         apply pow2_wneg.
-    Qed.
+    Qed. 
 
     Lemma RawFloat_RecFN_FN:
       evalExpr (isFiniteNonzero (getRawFloat_from_RecFN (getRecFN_from_FN fn))) = true ->
@@ -1364,6 +1335,7 @@ Section Properties.
         rewrite isNaN_or_Inf_infOrNaN.
         case_eq (evalExpr (infOrNaN fn)); intros sth2; simpl; auto.
         specialize (sth sth2).
+        assert (sth' : ZToWord 1 1 = natToWord 1 1) by auto; rewrite sth'; clear sth'.
         rewrite sth.
         auto.
       - simpl.
@@ -1375,7 +1347,7 @@ Section Properties.
         rewrite isNaN_or_Inf_infOrNaN.
         case_eq (evalExpr (infOrNaN fn)); intros sth2; simpl; auto.
         specialize (sth sth2); auto.
-        + unfold natToWord; simpl; rewrite sth.
+        + simpl; rewrite sth.
           rewrite andb_true_r.
           auto.
         + rewrite andb_false_r; simpl.
@@ -1432,7 +1404,7 @@ Section Properties.
             rewrite H.
             pose proof (@wzero_wones expWidth ltac:(lia)) as sth.
             simpl in *.
-            destruct (weq (wones expWidth) (natToWord expWidth 0)); simpl; auto.
+            destruct (weq _ (wones expWidth) (natToWord expWidth 0)); simpl; auto.
             rewrite e in *.
             tauto.
             Opaque infOrNaN isZeroExpIn.
@@ -1492,7 +1464,7 @@ Section Properties.
             rewrite H.
             pose proof (@wzero_wones expWidth ltac:(lia)) as sth.
             simpl in *.
-            destruct (weq (wones expWidth) (natToWord expWidth 0)); simpl; auto.
+            destruct (weq _ (wones expWidth) (natToWord expWidth 0)); simpl; auto.
             rewrite e in *.
             tauto.
             Opaque infOrNaN isZeroExpIn.
@@ -1532,6 +1504,7 @@ Section Properties.
         simpl in sth.
         case_eq (evalExpr (infOrNaN fn)); intros sth2; simpl; auto.
         + specialize (sth sth2); auto.
+          replace (ZToWord 1 0) with (natToWord 1 0); auto.
           rewrite sth.
           rewrite andb_true_r.
           auto.
@@ -1573,7 +1546,7 @@ Section Properties.
         * repeat econstructor; unfold key_not_In; intros; intro.
         * simpl; intros; tauto.
         * simpl; intros; tauto.
-        * do 8 f_equal; intros.
+        * do 8 f_equal; intros. 
           eapply  classifyImpl_correct.
         * intros.
           rewrite DisjKeyWeak_same by (apply string_dec).
